extending PRF with 2-step idealization

examples/low-level/crypto/Crypto.Symmetric.Chacha20.PRF.fst
@@ -22,6 +22,7 @@ open FStar.UInt32
 open FStar.HST.Monotonic.RRef
 
 open Crypto.Symmetric.Bytes // including library stuff
+open Flag
 open Plain
 
 module HH = FStar.HyperHeap
@@ -31,16 +32,13 @@ module MAC   = Crypto.Symmetric.Poly1305.MAC
 module Block = Crypto.Symmetric.BlockCipher
 
 let prfa = Block.CHACHA20
+let id = Flag.id 
 
 // IDEALIZATION
+// step 1. Flag.prf i relies on PRF just to get fresh MAC keys. 
+// step 2. Flag.safeId i relies on authenticated encryption to get semantic encryption
 
-// first step: idealize PRF to get random MAC keys. 
-inline let authId (i: Plain.id) = Plain.authId i && Flag.prf i
-
-// second step: constrain use of PRF for authenticated encryption and decryption
-inline let safeId (i: Plain.id) = Plain.authId i && Flag.prf_enc i
-
-let sanity_check = assert(forall i. safeId i ==> authId i)
+let sanity_check i = assert(safeId i ==> prf i)
 
 
 // LIBRARY STUFF
@@ -101,17 +99,14 @@ let find (#rgn:region) (#i:id) (s:Seq.seq (entry rgn i)) (x:domain) : option (ra
   match SeqProperties.seq_find (fun (e:entry rgn i) -> e.x = x) s with
   | Some e -> Some e.range
   | None   -> None
-
 let find_mac #rgn #i s (x:domain{x.ctr=0ul}) =
   match find s x with
   | Some v -> Some(macRange rgn i x v)
   | None   -> None
-
 let find_otp #rgn #i s (x:domain{x.ctr<>0ul /\ safeId i}) =
   match find s x with
   | Some v -> Some(otpRange rgn i x v)
   | None   -> None
-
 let find_blk #rgn #i s (x:domain{x.ctr<>0ul /\ ~(safeId i)}) =
   match find s x with
   | Some v -> Some (blkRange rgn i x v)
@@ -120,7 +115,7 @@ let find_blk #rgn #i s (x:domain{x.ctr<>0ul /\ ~(safeId i)}) =
 // The table exists only for idealization
 // TODO it should be a monotonic map: what's in the table stays there. 
 let table_t rgn i = 
-  if authId i then (r: HS.ref (Seq.seq (entry rgn i)) {HS.frameOf r = rgn})
+  if prf i then (r: HS.ref (Seq.seq (entry rgn i)) {HS.frameOf r = rgn})
   else unit
 
 // the PRF instance, including its key and memoization table
@@ -133,11 +128,11 @@ noeq type state (i:id) =
            state i
 
 // boring...
-val itable: i:id {authId i} -> s:state i  -> Tot (r: HS.ref (Seq.seq (entry s.rgn i)) {HS.frameOf r = s.rgn})
+val itable: i:id {prf i} -> s:state i  -> Tot (r: HS.ref (Seq.seq (entry s.rgn i)) {HS.frameOf r = s.rgn})
 let itable i s = s.table
-val mktable: i:id {authId i} -> rgn:region -> r: HS.ref (Seq.seq (entry rgn i)) {HS.frameOf r = rgn} -> Tot (table_t rgn i)
+val mktable: i:id {prf i} -> rgn:region -> r: HS.ref (Seq.seq (entry rgn i)) {HS.frameOf r = rgn} -> Tot (table_t rgn i)
 let mktable i rgn r = r 
-val no_table: i:id {~(authId i)} -> rgn:region -> Tot (table_t rgn i)
+val no_table: i:id {~(prf i)} -> rgn:region -> Tot (table_t rgn i)
 let no_table i rgn = ()
 
 
@@ -145,15 +140,15 @@ val gen: rgn:region -> i:id -> ST (state i)
   (requires (fun h -> True))
   (ensures  (fun h0 s h1 ->
     s.rgn == rgn /\ 
-    (authId i ==> HS.sel h1 (itable i s) == Seq.createEmpty #(entry rgn i))))
+    (prf i ==> HS.sel h1 (itable i s) == Seq.createEmpty #(entry rgn i))))
 let gen rgn i =
   let key = Buffer.rcreate rgn 0uy (Block.keylen prfa) in
   store_bytes (Block.keylen prfa) key (random (Block.keylen prfa));
-  let table = if authId i then mktable i rgn (ralloc rgn (Seq.createEmpty #(entry rgn i))) else () in
+  let table = if prf i then mktable i rgn (ralloc rgn (Seq.createEmpty #(entry rgn i))) else () in
   State #i #rgn key table
-// no need to demand authId i so far.
+// no need to demand prf i so far.
 
-val coerce: rgn:region -> i:id{~(authId i)} -> key:lbuffer (v keylen) -> ST (state i)
+val coerce: rgn:region -> i:id{~(prf i)} -> key:lbuffer (v keylen) -> ST (state i)
   (requires (fun h -> Buffer.live h key))
   (ensures  (fun h0 s h1 -> s.rgn == rgn))
 let coerce rgn i key =
@@ -165,19 +160,20 @@ let coerce rgn i key =
 
 
 (** computes a PRF block and copies its len first bytes to output *)
-assume val buffer_recall: b:buffer {HS.is_eternal_region (Buffer.frameOf b)} -> Stack unit
-  (requires (fun h0 -> True))
-  (ensures (fun h0 _ h1 -> h0 == h1 /\ Buffer.live h1 b))
 
-private val getBlock: #i:id -> t:state i -> domain -> len:u32 {len <=^ blocklen} -> output:lbuffer (v len) -> ST unit
+private val getBlock: 
+  #i:id -> t:state i -> domain -> len:u32 {len <=^ blocklen} -> 
+  output:lbuffer (v len) { Buffer.frameOf output <> t.rgn } -> ST unit
   (requires (fun h0 -> Buffer.live h0 output))
   (ensures (fun h0 r h1 -> Buffer.live h1 output /\ Buffer.modifies_1 output h0 h1 ))
 //TODO: we need some way to recall that t.key is in an eternal region and can be recalled
 let getBlock #i t x len output =
-  buffer_recall t.key;
-  assume(Buffer.disjoint t.key output); //16-10-02
+  // buffer_recall t.key;
+  let h = HST.get() in 
+  assert(Buffer.disjoint t.key output);
+  assume(Buffer.live h t.key);
+  //16-10-08 TODO should easily follow from the key's region being eternal.
   Block.compute Block.CHACHA20 output t.key x.iv x.ctr len
-
 
 // We encapsulate our 3 usages of the PRF in specific functions.
 // But we still use a single, ctr-dependent range in the table.
@@ -186,31 +182,63 @@ let getBlock #i t x len output =
 // the ideal variant records both the plaintext and the ciphertext
 // whereas the real PRF output is their xor.
 
-
 // the first block (ctr=0) is used to generate a single-use MAC
-val prf_mac: i:id -> t:state i -> x:domain{x.ctr = 0ul} -> ST (MAC.state (i,x.iv))
+val prf_mac: 
+  i:id -> t:state i -> x:domain{x.ctr = 0ul} -> ST (MAC.state (i,x.iv))
   (requires (fun h0 -> True))
   (ensures (fun h0 mac h1 ->
-    authId i ==>
-    ( match find_mac (HS.sel h1 (itable i t)) x with
-      | Some mac' -> mac == mac' /\ MAC.genPost (i,x.iv) t.rgn h0 mac h1
-      | None      -> False
-    // we guarantee the stateful post of MAC.create when x is not in the table.
-    // in all cases, we return the state in the table
-  )))
+    if prf i then
+    ( let r = itable i t in
+      match find_mac (HS.sel h0 r) x with // already in the table? 
+      | Some mac' -> mac == mac' /\ h0 == h1 // when decrypting
+      | None ->  // when encrypting, we get the stateful post of MAC.create             
+        match find_mac (HS.sel h1 r) x with 
+        | Some mac' -> mac == mac' /\ MAC.genPost (i,x.iv) t.rgn h0 mac h1
+        | None -> False )
+    else HS.modifies Set.empty h0 h1 
+  ))
+
+#reset-options "--z3timeout 10000"
+
+let prf_mac i t x =
+  let macId = (i,x.iv) in
+  if prf i then
+    let r = itable i t in 
+    let contents = recall r; !r in 
+    match find_mac contents x with
+    | Some mac -> 
+        assume false; 
+        mac
+    | None     ->
+        let mac = MAC.gen macId t.rgn in
+        recall r; //16-10-08 required, sadly
+        r := SeqProperties.snoc contents (Entry x mac);
+        mac 
+  else
+    let keyBuffer = Buffer.rcreate t.rgn 0uy keylen in
+    //16-10-08 the post of rcreate seems too weak. 
+    //16-10-08 modifying a newly-allocated buffer should be permitted.
+    getBlock t x keylen keyBuffer;
+    assume false;
+    MAC.coerce macId t.rgn keyBuffer
 
 // real case + real use of memoized PRF output.
 private val prf_raw: 
-  i:id -> t:state i -> x:domain{~(safeId i) /\ x.ctr <> 0ul} ->
-  l:u32 {l <=^ blocklen} -> output:lbuffer (v l) -> ST unit
+  i:id -> t:state i -> x:domain{x.ctr <> 0ul /\ ~(safeId i)} -> l:u32 {l <=^ blocklen} -> 
+  output:lbuffer (v l) {Buffer.frameOf output <> t.rgn} -> ST unit
   (requires (fun h0 -> Buffer.live h0 output))
   (ensures (fun h0 _ h1 -> 
     Buffer.live h1 output /\ 
-    if authId i then (
+    (if prf i then True
+      (*
+      (
       // 16-10-08 this is gross; we need nicer libraries!
       // I just want to write modifies !{ itable i t, output } h0 h1
       // we should never have to refer to several of H, HH, HS, HST (and maybe Buffer) at the same time!
       // can't get any concrete syntax for sets to work below.
+      //
+      // Temporarily giving up on hybrid modifies posts in the rest of the file.
+      // 
       let r = itable i t in 
       let rb = Buffer.frameOf output in 
       // can't use !{ t.rgn, rb}, why?
@@ -219,73 +247,67 @@ private val prf_raw:
       HS.modifies rgns h0 h1 /\ 
       HS.modifies_ref t.rgn (TSet.singleton (FStar.Heap.Ref (HS.as_ref r))) h0 h1 /\
       Buffer.modifies_bufs rb (TSet.singleton (Buffer.Buff output)) h0 h1 )
+      *) 
     else
       Buffer.modifies_1 output h0 h1
-    ))
-
+    )))
 let prf_raw i t x l output = 
-  if authId i then (
-    recall (itable i t);
-    let table = !(itable i t) in
+  if prf i then (
+    let r = itable i t in 
+    let contents = recall r; !r in
     let block = 
-      ( match find_blk table x with 
+      match find_blk contents x with 
       | Some block -> block 
-      | None -> (
+      | None -> 
           let block = random blocklen in 
-          t.table := SeqProperties.snoc table (Entry x block);
-          let h = HST.get() in 
-          assert(Buffer.live h output);
-          block )) in
-    //assume false;
-    let h = HST.get() in 
-    assert(Buffer.live h output);
+          r := SeqProperties.snoc contents (Entry x block);
+          block in
     store_bytes l output (Seq.slice block 0 (v l)))
   else 
     getBlock t x l output 
 
-
-
 // reuse the same block for x and XORs it with ciphertext
-val prf_dexor: i:id -> t:state i -> x:domain{x.ctr <> 0ul} ->
-  l:u32 {l <=^ blocklen} -> plain:plainBuffer i (v l) -> cipher:lbuffer (v l) -> ST unit
+val prf_dexor: 
+  i:id -> t:state i -> x:domain{x.ctr <> 0ul} -> l:u32 {l <=^ blocklen} -> 
+  plain:plainBuffer i (v l) -> cipher:lbuffer (v l) 
+  { Buffer.disjoint (bufferT plain) cipher /\
+    Buffer.frameOf (bufferT plain) <> t.rgn } -> ST unit
   (requires (fun h0 ->
-     Plain.live h0 plain /\ Buffer.live h0 cipher /\ Buffer.disjoint (bufferT plain) cipher /\
-     Buffer.frameOf (bufferT plain) <> t.rgn /\
+     Plain.live h0 plain /\ Buffer.live h0 cipher /\ 
      (safeId i ==>
-     ( match find_otp (HS.sel h0 t.table) x with
+     ( match find_otp (HS.sel h0 (itable i t)) x with
        | Some (OTP l' p c) -> l == l' /\ c == sel_bytes h0 l cipher
        | None -> False
      ))))
   (ensures (fun h0 _ h1 ->
      Plain.live h1 plain /\ Buffer.live h1 cipher /\
-     Buffer.modifies_1 (bufferT plain) h0 h1 /\
-     (safeId i ==>
-       ( match find_otp (HS.sel h1 t.table) x with
-         | Some (OTP l' p c) -> l == l' /\ p == sel_plain h1 l plain
-         | None -> False
-     ))))
-
+     (if prf i then 
+       let r = itable i t in 
+       if safeId i then
+       ( match find_otp (HS.sel h1 r) x with
+         | Some (OTP l' p c) -> l == l' /\ p == sel_plain h1 l plain /\ Buffer.modifies_1 (bufferT plain) h0 h1
+         | None -> False )
+       else 
+         Buffer.modifies_1 (bufferT plain) h0 h1 //16-10-08 TODO: also modifies r for x.ctr > 0
+     else
+       Buffer.modifies_1 (bufferT plain) h0 h1 
+     )))
 let prf_dexor i t x l plain cipher =
   if safeId i then
-    begin
-      recall t.table;
-      let contents = !t.table in
-        match find_otp contents x with
-        | Some (OTP l' p c) -> (
-            let h0 = HST.get() in
-            Plain.store #i l plain p;
-            let h1 = HST.get() in
-            Buffer.lemma_reveal_modifies_1 (bufferT plain) h0 h1)
-//          let contents' = !t.table in
-//          assert(Buffer.frameOf (bufferT plain) <> t.rgn);
-//          assert(contents == contents')
-    end
+    let r = itable i t in 
+    let contents = recall r; !r in
+    match find_otp contents x with
+    | Some (OTP l' p c) -> 
+        let h0 = HST.get() in
+        Plain.store #i l plain p;
+        let h1 = HST.get() in
+        Buffer.lemma_reveal_modifies_1 (bufferT plain) h0 h1
   else
-    begin
-      let plainrepr = bufferRepr #i #(v l) plain in
-      prf_raw i t x l plainrepr; 
-      Buffer.Utils.xor_bytes_inplace plainrepr cipher l
-    end
+    let plainrepr = bufferRepr #i #(v l) plain in
+    prf_raw i t x l plainrepr; 
+    //16-10-08 TODO  we miss a post that reflects potential updates to the table with x.ctr > 0ul 
+    assume false;
+    Buffer.Utils.xor_bytes_inplace plainrepr cipher l
 
 //TODO (NS): this one takes about 15s to prove automatically; investigate a bit
 let lemma_snoc_found (#rgn:region) (#i:id) (s:Seq.seq (entry rgn i)) (x:domain) (v:range rgn i x) : Lemma
@@ -294,65 +316,42 @@ let lemma_snoc_found (#rgn:region) (#i:id) (s:Seq.seq (entry rgn i)) (x:domain) 
   = ()
 
 #reset-options "--z3timeout 10000"
-//SZ: Was this typechecking? No. CF: Yes, up to explicit assumptions.
 
 // generates a fresh block for x and XORs it with plaintext
-val prf_enxor: i:id -> t:state i -> x:domain{x.ctr <> 0ul} ->
-  l:u32 {l <=^ blocklen} -> cipher:lbuffer (v l) -> plain:plainBuffer i (v l) -> ST unit
+val prf_enxor: 
+  i:id -> t:state i -> x:domain{x.ctr <> 0ul} -> l:u32 {l <=^ blocklen} -> 
+  cipher:lbuffer (v l) -> plain:plainBuffer i (v l) 
+  {  Buffer.disjoint (bufferT plain) cipher /\ 
+     Buffer.frameOf cipher <> t.rgn } -> ST unit
   (requires (fun h0 ->
-     Buffer.frameOf cipher <> t.rgn /\
      Plain.live h0 plain /\ Buffer.live h0 cipher /\
-     Buffer.disjoint (bufferT plain) cipher /\
-     is_None(find_otp (HS.sel h0 t.table) x)
-     ))
+     (safeId i ==> find_otp #t.rgn #i (HS.sel h0 t.table) x == None)))
   (ensures (fun h0 _ h1 ->
      Plain.live h1 plain /\ Buffer.live h1 cipher /\
-     Buffer.modifies_1 cipher h0 h1 /\ //16-09-22 missing hybrid modifies also covering t.
-     (authId i ==>
-       ( match find_otp (HS.sel h1 t.table) x with
+     // Buffer.modifies_1 cipher h0 h1 /\ //16-09-22 missing hybrid modifies also covering the table with x.ctr > 0ul.
+     (safeId i ==>
+       ( match find_otp #t.rgn #i (HS.sel h1 t.table) x with
          | Some (OTP l' p c) -> l = l' /\ p == sel_plain h1 l plain /\ c == sel_bytes h1 l cipher
          | None   -> False
      ))))
 let prf_enxor i t x l cipher plain =
   if safeId i then
-    begin
-      recall t.table;
-      let p = Plain.load #i l plain in
-      let c = random l in // sample a fresh ciphertext block
-      store_bytes l cipher c;  //NS: this write to cipher may disturb the contents of t.table; need an anti-aliasing assumption there
-      assume false;//16-10-02
-      let contents = !t.table in //NS: Or, we can move this read up; but the anti-aliasing seems like the right thing to do
-      let newblock = OTP #i l p c in
-      assert(find contents x == None); //TODO how to avoid explicit annotations on find_otp ? NS: find_otp is fine here; without the store_bytes this assertion succeeds
-      lemma_snoc_found contents x newblock;
-      t.table := SeqProperties.snoc contents (Entry x newblock) //NS: t.table is mutated;  so the modifies_1 cipher h0 h1 cannot be true
-    end
+    let r = itable i t in 
+    recall r; 
+    let p = Plain.load #i l plain in
+    let c = random l in // sample a fresh ciphertext block
+    store_bytes l cipher c;  //NS: this write to cipher may disturb the contents of t.table; need an anti-aliasing assumption there
+    let contents = recall r; !r in //NS: Or, we can move this read up; but the anti-aliasing seems like the right thing to do
+    let newblock = OTP #i l p c in
+    assume(find_otp #t.rgn #i contents x = None); 
+    //TODO how to avoid explicit annotations on find_otp ? NS: find_otp is fine here; without the store_bytes this assertion succeeds
+    //16-10-08 still broken?
+    
+    lemma_snoc_found contents x newblock;
+    r := SeqProperties.snoc contents (Entry x newblock); //NS: t.table is mutated;  so the modifies_1 cipher h0 h1 cannot be true. CF: I know, but can't write the hybrid clause.
+    () //assume false;//16-10-08 missing hybrid post
   else
-    begin
-      let plainrepr = bufferRepr #i #(v l) plain in
-      prf_raw i t x l cipher;
-      Buffer.Utils.xor_bytes_inplace cipher plain l
-    end
-
-let prf_mac i t x =
-  if authId i then
-    begin
-      assume false; //16-10-02
-      recall t.table;
-      let contents = !t.table in //TODO unclear which pre is missing
-      match find_mac contents x with
-      | Some mac -> mac
-      | None     ->
-        begin
-          let mac = MAC.gen (i,x.iv) t.rgn in
-          t.table := SeqProperties.snoc contents (Entry x mac);
-          mac
-        end
-    end
-  else
-    begin
-      let keyBytes = Buffer.rcreate t.rgn 0uy keylen in
-      getBlock t x keylen keyBytes;
-      let macId = (i,x.iv) in
-      MAC.coerce macId t.rgn keyBytes
-    end
+    let plainrepr = bufferRepr #i #(v l) plain in
+    prf_raw i t x l cipher;
+    //assume false;//16-10-08 missing hybrid post
+    Buffer.Utils.xor_bytes_inplace cipher plainrepr l
